src/tls/StreamAE.fst
@@ -9,6 +9,7 @@ module HST = FStar.HyperStack.ST //Added automatically
 module HS = FStar.HyperStack 
 
 module I = Crypto.Indexing
+module U8 = FStar.UInt8
 module U32 = FStar.UInt32
 module U64 = FStar.UInt64
 module U128 = FStar.UInt128
@@ -30,7 +31,10 @@ open TLSError
 open TLSConstants
 open TLSInfo
 
+#reset-options "--initial_fuel 1 --max_fuel 1 --z3rlimit 50"
+
 type plainLenMin = AEAD.plainLenMin 1
+type iplainLenMin = l:AEAD.plainLenMin 1{l + v AEAD.taglen < pow2 32 - 1}
 
 // plain i lmax: stream plaintext of length at most lmax
 let plain i lmax = llbytes lmax
@@ -41,7 +45,7 @@ type aead_plain (i:I.id) (l:plainLenMin) : t:Type0{hasEq t} = lbytes l
 
 type counter = c:UInt32.t{UInt32.v c <= max_ctr}
 
-let increases_u32 (x:U32.t) (y:U32.t)  = b2t (x <=^ y)
+let increases_u32 (x:U32.t) (y:U32.t)  = increases (v x) (v y)
 
 let ctr_ref (r:erid) (i:I.id) : Tot Type0 =
   m_rref r counter increases_u32
@@ -66,8 +70,64 @@ let aead_plain_pkg = AEAD.PlainPkg 1 aead_plain as_bytes repr
 type aead_info (i:I.id) = u:(AEAD.info i){u.AEAD.plain == aead_plain_pkg}
 
 
-assume val pad: lmax:plainLen -> p:llbytes lmax -> lbytes (lmax+1)
-assume val unpad: #l:plainLenMin -> p:lbytes l -> llbytes (l-1)
+val pad: lmax:plainLen -> p:llbytes lmax -> lbytes (lmax+1)
+let pad lmax p =
+  let lz = U32.uint_to_t (lmax - (length p)) in
+  let z = Bytes.create lz (U8.uint_to_t 0) in
+  let one = Bytes.create 1ul (U8.uint_to_t 1) in
+  Bytes.append (Bytes.append p one) z
+  
+
+val unpad: #l:plainLenMin -> p:lbytes l -> llbytes (l-1)
+let rec unpad #l p =
+  let last = U32.uint_to_t (l - 1) in
+  let pp = Bytes.slice p 0ul last in
+  if Bytes.get p last = U8.uint_to_t 0 && l > 1 then
+    let ppp = unpad #(l-1) pp <: bytes in
+    ppp
+  else
+    pp
+
+val unpad_zero (l:plainLenMin{l>=2}) (p:lbytes (l-1)) : Lemma
+  (requires True)
+  (ensures
+    (unpad #l (Bytes.append p (Bytes.create 1ul (U8.uint_to_t 0)))) = 
+    (unpad #(l-1) p <: bytes))
+let unpad_zero l p =
+  let zero = U8.uint_to_t 0 in
+  let zerob = Bytes.create 1ul zero in
+  let last = U32.uint_to_t (l - 1) in
+  let p' = Bytes.append p zerob in
+  let pp = Bytes.slice p' 0ul last in
+  Seq.Base.lemma_eq_elim (Bytes.reveal p) (Bytes.reveal pp)
+  
+val unpad_pad (lmax:plainLen) (p:llbytes lmax) : Lemma
+  (requires True)
+  (ensures
+    unpad (pad lmax p) = p)
+
+let rec unpad_pad lmax p = 
+  let zero = U8.uint_to_t 0 in
+  let zerob = Bytes.create 1ul zero in
+  let one = U8.uint_to_t 1 in
+  let oneb = Bytes.create 1ul one in 
+  let last = U32.uint_to_t lmax in
+  let pp = Bytes.slice (pad lmax p) 0ul last in
+  if lmax - length p = 0 then
+    (//    assert (pad lmax p = Bytes.append p oneb);
+//    assert (Bytes.get (pad lmax p) last = one);
+    Seq.Base.lemma_eq_elim (Bytes.reveal pp) (Bytes.reveal p))
+  else
+    (Seq.Base.lemma_eq_elim (Bytes.reveal (pad lmax p)) (Bytes.reveal (Bytes.append (pad (lmax - 1) (p <: bytes)) (zerob)));
+ //   assert (length p <= lmax - 1);
+//    assert (pad lmax p = Bytes.append (pad (lmax - 1) p) (zerob));
+    unpad_zero (lmax+1) (pad (lmax - 1) (p <: bytes));
+//    assert (unpad (pad lmax p) = unpad (pad (lmax - 1) (p <: bytes)));
+    unpad_pad (lmax - 1) (p <: bytes))
+
+  
+
+  
 
 let plain_of_aead_plain
   (#i:I.id)
@@ -113,7 +173,11 @@ noeq type stream_reader (#i:I.id) (w:stream_writer i) =
     #region: rgn ->
     aead: AEAD.aead_reader (Stream_writer?.aead w)
       {(AEAD.rgetinfo aead).AEAD.plain == aead_plain_pkg /\
-      ~ (Set.mem region (Set.union (AEAD.rfootprint aead) (AEAD.shared_footprint)))} ->
+        Set.disjoint (Set.singleton region) (AEAD.wfootprint (Stream_writer?.aead w)) /\
+        Set.disjoint (Set.singleton region) (AEAD.rfootprint aead) /\
+        Set.disjoint (Set.singleton region) (AEAD.shared_footprint) /\
+        Set.disjoint (Set.singleton region) (Set.singleton (Stream_writer?.region w)) /\
+        Set.disjoint (Set.singleton (Stream_writer?.region w)) (AEAD.rfootprint aead)} ->
     iv: AEAD.iv (I.cipherAlg_of_id i){iv = w.iv} ->
     ctr: ctr_ref region i ->
     stream_reader w
@@ -143,7 +207,7 @@ let invariant (#i:I.id) (w:stream_writer i) (h:mem) =
     let wlg = AEAD.wlog (Stream_writer?.aead w) h in
     let iv = Stream_writer?.iv w in
     UInt32.v wc = Seq.length wlg /\
-    (forall (j:U32.t). (v j < v wc) ==> AEAD.Entry?.nonce (Seq.index wlg (v j)) = create_nonce iv j)
+    (forall (j:nat). (j < Seq.length wlg) ==> AEAD.Entry?.nonce (Seq.index wlg j) = create_nonce iv (U32.uint_to_t j))
   else
     True)
 
@@ -154,7 +218,7 @@ let rinvariant (#i:I.id) (#w:stream_writer i) (r:stream_reader w) (h:mem) =
   let wc = sel h (Stream_writer?.ctr w) in
   let rc = sel h (Stream_reader?.ctr r) in
   AEAD.winvariant (Stream_writer?.aead w) h /\
-  rc <=^ wc
+  (safeId i ==> rc <=^ wc)
 
 let wctrT (#i:I.id) (w:stream_writer i) (h:mem) =
   v (sel h (Stream_writer?.ctr w)) 
@@ -175,7 +239,11 @@ let stream_entry_of_aead_entry (#i:I.id) (#u:aead_info i) (e:AEAD.entry i u) =
     | AEAD.Entry nonce ad #l p c ->
       Entry ad (plain_of_aead_plain p) (cipher_of_aead_cipher c)
 
-let seqmap (#t:Type) (#t':Type) (f:(t -> t')) (s:seq t) : (s':seq t'{Seq.length s = Seq.length s'}) =
+let seqmap (#t:Type) (#t':Type) (f:(t -> t')) (s:seq t) : 
+  (s':seq t'
+    {Seq.length s = Seq.length s' /\ 
+    (forall (i:nat). i < Seq.length s ==> Seq.index s' i == f (Seq.index s i))})
+  =
   Seq.init (Seq.length s) (fun j -> f (Seq.index s j))
 
 let wlog (#i:safeid) (w:stream_writer i) (h:mem) =
@@ -233,7 +301,7 @@ let lem_ivlen alg = ()
 let rec little_endian (b:bytes) : Tot (n:nat) (decreases (length b)) =
   if length b = 0 then 0
   else
-    let b' = sub b 1ul (U32.uint_to_t ((length b) - 1)) in
+    let b' = slice b 1ul (U32.uint_to_t (length b)) in
     let h = FStar.Bytes.get b 0ul in
     (UInt8.v h) + pow2 8 * little_endian b'
 
@@ -245,30 +313,43 @@ let lemma_euclidean_division r b q = ()
 val lemma_factorise: a:nat -> b:nat -> Lemma (a + a * b == a * (b + 1))
 let lemma_factorise a b = ()
 
+val lemma_mult_le_left': a:nat -> b:int -> c:int -> Lemma
+  (requires (b <= c))
+  (ensures  (a * b <= a * c))
+let lemma_mult_le_left' a b c = ()
+
+
+val lemma_mult_lt_left': a:pos -> b:int -> c:int -> Lemma
+  (requires (b < c))
+  (ensures  (a * b < a * c))
+let lemma_mult_lt_left' a b c = ()
+
 val lemma_little_endian_is_bounded: b:bytes -> Lemma
   (requires True)
-  (ensures  (little_endian b < pow2 (8 * length b)))
+  (ensures little_endian b < pow2 (8 * length b))
   (decreases (length b))
 let rec lemma_little_endian_is_bounded b =
   if length b = 0 then ()
   else
-    admit()
-
-(*
     begin
     let s = slice b 1ul (U32.uint_to_t (length b)) in
     assert(length s = length b - 1);
     lemma_little_endian_is_bounded s;
     assert(UInt8.v (FStar.Bytes.get b 0ul) < pow2 8);
     assert(little_endian s < pow2 (8 * length s));
+    lemma_mult_lt_left' (pow2 8) (little_endian s) (pow2 (8 * length s));
+    assert(pow2 8 * little_endian s < pow2 8 * pow2 (8 * length s));    
+    assert (little_endian b = (UInt8.v (FStar.Bytes.get b 0ul)) + pow2 8 * little_endian s);
     assert(little_endian b < pow2 8 + pow2 8 * pow2 (8 * (length b - 1)));
     lemma_euclidean_division (UInt8.v (FStar.Bytes.get b 0ul)) (little_endian s) (pow2 8);
+    assert (little_endian s + 1 <= pow2 (8 * (length b - 1)));
     assert(little_endian b <= pow2 8 * (little_endian s + 1));
+    lemma_mult_le_left' (pow2 8) (little_endian s+1) (pow2 (8 * (length b - 1)));
     assert(little_endian b <= pow2 8 * pow2 (8 * (length b - 1)));
     Math.Lemmas.pow2_plus 8 (8 * (length b - 1));
     lemma_factorise 8 (length b - 1)
     end
-*)
+
 
 val uint8_to_uint128: a:UInt8.t -> Tot (b:UInt128.t{UInt128.v b == UInt8.v a})
 let uint8_to_uint128 a = U128.uint64_to_uint128 (FStar.Int.Cast.uint8_to_uint64 a)
@@ -276,20 +357,21 @@ let uint8_to_uint128 a = U128.uint64_to_uint128 (FStar.Int.Cast.uint8_to_uint64 
 
 val load_uint128:
   alg:I.cipherAlg ->
-  len:U32.t {len <=^ (AEAD.ivlen alg)} -> 
+  len:U32.t {v len <= v (AEAD.ivlen alg)} -> 
   b:lbytes (v len) -> 
   Tot (n:U128.t{U128.v n == little_endian b}) (decreases (v len))
-  
+
+
+
 let rec load_uint128 alg len b =
   if len = 0ul then U128.uint64_to_uint128 0UL
   else
-    let n' = load_uint128 alg (len -^ 1ul) (sub b 1ul (len -^ 1ul)) in
+    let n' = load_uint128 alg (len -^ 1ul) (slice b 1ul len) in
     let h = FStar.Bytes.get b 0ul in
-    lemma_little_endian_is_bounded
-      (sub b 1ul (len -^ 1ul));
-     magic()
-(*    assert (UInt128.v n' <= pow2 (8 * v len - 8) - 1);
-   assert (256 * UInt128.v n' <= 256 * pow2 (8 * v len - 8) - 256);
+    lemma_little_endian_is_bounded (slice b 1ul len);
+    assert (UInt128.v n' <= pow2 (8 * v len - 8) - 1);
+    lemma_mult_le_left' (256) (U128.v n') (pow2 (8 * v len - 8) - 1);
+    assert (256 * UInt128.v n' <= 256 * pow2 (8 * v len - 8) - 256);
     assert_norm (256 * pow2 (8 * 16 - 8) - 256 <= pow2 128 - 256);
     Math.Lemmas.pow2_le_compat (8 * 16 - 8) (8 * v len - 8);
     assert (256 * pow2 (8 * v len - 8) - 256 <= pow2 128 - 256);
@@ -297,52 +379,335 @@ let rec load_uint128 alg len b =
     assert_norm (pow2 (UInt32.v 8ul) == 256);
     assert (256 * UInt128.v n' == FStar.UInt128.(v (n' <<^ 8ul)));
     FStar.UInt128.(uint8_to_uint128 h +^ (n' <<^ 8ul))
-*)
 
-//parent in the info ?
-let create (parent:rgn) (i:I.id) (u:info i) =
-  let w = AEAD.gen i (aead_info_of_info u) in
-  let rr = new_region parent in
-  let alg = I.cipherAlg_of_aeadAlg u.alg in
+let random_iv (alg:I.cipherAlg) :
+  ST (AEAD.iv alg) (requires fun _ -> True) (ensures fun h0 _ h1 -> h0 == h1) =
   let ivlen = AEAD.ivlen alg in
   let b = CoreCrypto.random32 ivlen in
   let iv = load_uint128 alg ivlen b in
-  let ctr = ralloc #(U32.t) #increases_u32 rr 0ul in
-  admit();
-  Stream_writer #i #rr w iv ctr
+  lemma_little_endian_is_bounded b;
+  iv
+
+
+
+assume val frame_invariant': #i:I.id -> w:stream_writer i -> h0:mem -> h1:mem ->
+  Lemma
+  (requires
+    (invariant w h0 /\
+    modifies_none h0 h1 ))
+  (ensures invariant w h1)
+
+assume val aead_frame_invariant': #i:I.id -> w:AEAD.aead_writer i -> h0:mem -> h1:mem ->
+  Lemma
+  (requires
+    (AEAD.winvariant w h0 /\
+    modifies_none h0 h1 ))
+  (ensures AEAD.winvariant w h1)
+
+assume val aead_frame_log': #i:I.id -> w:AEAD.aead_writer i ->
+  h0:mem -> h1:mem ->
+  Lemma
+    (requires
+      safeId i /\
+      modifies_none h0 h1)
+    (ensures AEAD.wlog w h0 == AEAD.wlog w h1)
+  
+let create (i:I.id) (u:info i) = 
+  let w = AEAD.gen i (aead_info_of_info u) in
+  let h0 = get() in
+  let rr = new_region u.parent in
+  let alg = I.cipherAlg_of_aeadAlg u.alg in
+  let iv :AEAD.iv (I.cipherAlg_of_id i) = random_iv alg in
+  let ctr :ctr_ref rr i = ralloc #(U32.t) #increases_u32 rr 0ul in
+  let h1 = get() in
+  aead_frame_invariant' w h0 h1;
+  if safeId i then aead_frame_log' w h0 h1;
+  let s =   Stream_writer #i #rr w iv ctr in
+  if safeId i then Seq.Base.lemma_empty (wlog s h1);
+  s
   
 
-let coerce parent i u = admit()
+
+let coerce i u = admit()
 
 
-let createReader (parent:rgn) (#i:I.id) (w:stream_writer i) =
+let createReader (parent:rgn) (#i:I.id) (w:stream_writer i) = //:
+  let h0 = get() in
   let aw = Stream_writer?.aead w in
   let r = AEAD.genReader aw in
   let rr = new_region parent in
-  let iv = U128.uint_to_t 0 in
+  let iv = Stream_writer?.iv w in
   let ctr = ralloc #(U32.t) #increases_u32 rr 0ul in
-  admit()//;
-//  Stream_reader #i #w #rr r iv ctr 
+  assume ((Stream_writer?.region w) <> (AEAD.rgetinfo r).AEAD.prf_rgn); 
+  assume (~ (Set.mem rr 
+    (Set.union 
+      (Set.union 
+        (Set.union (AEAD.wfootprint aw) (AEAD.rfootprint r))
+        (Set.singleton (Stream_writer?.region w)))
+      (AEAD.shared_footprint))));
+  let h1 = get() in  
+  frame_invariant' w h0 h1;
+  Stream_reader #i #w #rr r iv ctr
 
 
-let encrypt #i (w:stream_writer i) ad lmax (p:plain i lmax) =
-  let pp:aead_plain i (lmax+1) = pad lmax p in
+
+val seqmap_snoc (#t:Type) (#t':Type) (s:Seq.seq t) (f:t -> t') (x:t) :
+  Lemma
+    (requires True)
+    (ensures seqmap f (Seq.snoc s x) == Seq.snoc (seqmap f s) (f x))
+let seqmap_snoc #t #t' s f x = 
+  Seq.Base.lemma_eq_elim (seqmap f (Seq.snoc s x)) (Seq.snoc (seqmap f s) (f x))
+
+//#reset-options "--initial_fuel 2 --max_fuel 2 --z3rlimit 10"
+
+
+val create_nonce_inj (#i:I.id) (iv:AEAD.iv (I.cipherAlg_of_id i)) (j:U32.t) (j':U32.t) :
+  Lemma
+  (requires create_nonce iv j = create_nonce iv j')
+  (ensures j = j')
+let create_nonce_inj #i iv j j' = 
+  FStar.UInt.logxor_associative #128 (U128.v iv) (U128.v iv) (U128.v (uint32_to_uint128 j));
+  FStar.UInt.logxor_associative #128 (U128.v iv) (U128.v iv) (U128.v (uint32_to_uint128 j'));
+  FStar.UInt.logxor_self #128 (U128.v iv);
+  FStar.UInt.logxor_commutative (UInt.zero 128) (U128.v (uint32_to_uint128 j));
+  FStar.UInt.logxor_commutative (UInt.zero 128) (U128.v (uint32_to_uint128 j'));
+  FStar.UInt.logxor_lemma_1 #128 (U128.v (uint32_to_uint128 j));
+  FStar.UInt.logxor_lemma_1 #128 (U128.v (uint32_to_uint128 j'))
+
+let create_nonce_inj' i iv j j' : Lemma ((create_nonce iv j = create_nonce iv j') ==> (j = j')) =
+(FStar.Classical.move_requires (create_nonce_inj #i iv j) j')
+
+let create_nonce_inj'' i iv j :
+Lemma (forall (j':U32.t). (create_nonce iv j = create_nonce iv j') ==> (j = j')) =  
+ FStar.Classical.forall_intro (fun j' -> create_nonce_inj' i iv j j')
+
+
+val lem_fresh (i:I.id) (w:stream_writer i) (h:mem) :
+  Lemma
+  (requires safeId i /\ wincrementable w h /\ invariant w h)
+  (ensures 
+   (let iv = Stream_writer?.iv w in
+    let aw = Stream_writer?.aead w in
+    AEAD.fresh_nonce (create_nonce iv (U32.uint_to_t (wctrT w h))) aw h))
+
+let lem_fresh i w h =
+  let iv = Stream_writer?.iv w in
+  let aw = Stream_writer?.aead w in
+  let n' = create_nonce iv (U32.uint_to_t (wctrT w h)) in
+  let lg = AEAD.wlog aw h in
+  match AEAD.wentry_for_nonce n' aw h with
+  | None -> ()
+  | Some e ->
+    lemma_find_l_contains (AEAD.nonce_filter #i #aw n') lg;
+    Seq.contains_elim lg e;
+    create_nonce_inj'' i iv (U32.uint_to_t (wctrT w h))
+//    assert (Seq.contains lg e);
+//    assert (AEAD.Entry?.nonce e = n');
+//    assert (exists (j:nat). j < Seq.length lg /\ n' = create_nonce iv (U32.uint_to_t j))
+  
+
+
+//#reset-options "--initial_fuel 1 --max_fuel 1 --z3rlimit 50"
+
+let encrypt
+  (#i:I.id) (w:stream_writer i) (ad:AEAD.adata) (lmax:plainLen) (p:plain i lmax) 
+=
+  let h0 = get() in
+  let pp = aead_plain_of_plain p in
   let aw = Stream_writer?.aead w in
   let ctr = Stream_writer?.ctr w in
-  let n = create_nonce (Stream_writer?.iv w) !ctr in
- // let cc:AEAD.cipher i (AEAD.wgetinfo aw) (lmax+1) = AEAD.encrypt i aw n ad (lmax+1) pp in
-//  let c = cipher_of_aead_cipher cc in
-  ctr := !ctr  + 1
-  admit() //c
+  let iv = Stream_writer?.iv w in
+  let n = create_nonce iv !ctr in
+  assert (safeId i ==> (forall (j:nat). (j < wctrT w h0) ==>
+    AEAD.Entry?.nonce (Seq.index (AEAD.wlog aw h0) j) = 
+    create_nonce iv (U32.uint_to_t j)));
+  if safeId i then lem_fresh i w h0;
+  let cc = AEAD.encrypt i aw n ad (lmax+1) pp in
+  let h05 = get() in
+  let c = cipher_of_aead_cipher cc in
+  ctr := !ctr +^ 1ul;
+  let h1 = get() in
+  AEAD.wframe_invariant aw h05 (Stream_writer?.region w) h1;
+  if safeId i then
+    begin
+      AEAD.frame_log aw (AEAD.wlog aw h05) h05 (Stream_writer?.region w) h1;
+      //AEAD.frame_log aw (Seq.snoc (AEAD.wlog aw h0) (AEAD.Entry n ad pp cc)) h05 (Stream_writer?.region w) h1;
+    //assert (AEAD.wlog aw h1 == 
+     // (Seq.snoc (AEAD.wlog aw h0) (AEAD.Entry n ad pp cc)));
+     seqmap_snoc (AEAD.wlog aw h0) stream_entry_of_aead_entry (AEAD.Entry n ad pp cc);
+    //assert (wlog w h1 == 
+      //(Seq.snoc (wlog w h0) (stream_entry_of_aead_entry (AEAD.Entry n ad pp cc))))
+    assert (forall (j:nat). (j <= wctrT w h0) ==>
+     AEAD.Entry?.nonce (Seq.index (AEAD.wlog aw h1) j) = 
+     create_nonce iv (U32.uint_to_t j))
+    end;
+  unpad_pad lmax p;
+//  assert (stream_entry_of_aead_entry (AEAD.Entry n ad pp cc) == Entry ad p c);
+  c
 
 
-let decrypt #i (#w:stream_writer i) (r:stream_reader w) ad lmax (c:cipher i lmax) =
+
+
+assume val aead_frame_log'': #i:I.id -> w:AEAD.aead_writer i ->
+  h0:mem -> s:rset -> h1:mem ->
+  Lemma
+    (requires
+      Set.disjoint s (AEAD.wfootprint w) /\
+      safeId i /\
+      modifies s h0 h1)
+    (ensures AEAD.wlog w h0 == AEAD.wlog w h1)
+ 
+
+val lem_nonce (i:I.id) (w:stream_writer i) (j:nat) (h:mem) :
+  Lemma
+  (requires safeId i /\ invariant w h /\ j < wctrT w h)
+  (ensures
+    (let wlg = wlog w h in
+    let aw = Stream_writer?.aead w in
+    let awlg = AEAD.wlog aw h in
+    let n = create_nonce (Stream_writer?.iv w) (U32.uint_to_t j) in
+    let u = AEAD.wgetinfo aw in
+    match Seq.index wlg j, Seq.index awlg j with
+      | Entry ad #lmax p c, AEAD.Entry n' ad' #l p' c' ->
+        n' == n /\
+        ad' == ad /\
+        plain_of_aead_plain #i #l p' == p /\
+        cipher_of_aead_cipher c' == c /\
+        l = lmax + 1))
+let lem_nonce i w j h = 
+  let wlg = wlog w h in
+  let aw = Stream_writer?.aead w in
+  let awlg = AEAD.wlog aw h in
+  let n = create_nonce (Stream_writer?.iv w) (U32.uint_to_t j) in
+  let u = AEAD.wgetinfo aw in
+  assert (stream_entry_of_aead_entry (Seq.index awlg j) == Seq.index wlg j)
+
+
+val lem_nonce2 (i:I.id) (w:stream_writer i) (j:nat) (h:mem) :
+  Lemma
+  (requires safeId i /\ invariant w h /\ j < wctrT w h)
+  (ensures
+    (let wlg = wlog w h in
+    let aw = Stream_writer?.aead w in
+    let awlg = AEAD.wlog aw h in
+    let n = create_nonce (Stream_writer?.iv w) (U32.uint_to_t j) in
+    let u = AEAD.wgetinfo aw in
+    match AEAD.wentry_for_nonce #i n aw h with
+      | Some e -> Seq.index awlg j = e
+      | None -> False))
+let lem_nonce2 i w j h = 
+  let wlg = wlog w h in
+  let aw = Stream_writer?.aead w in
+  let awlg = AEAD.wlog aw h in
+  let iv = Stream_writer?.iv w in
+  let n = create_nonce iv (U32.uint_to_t j) in
+  let u = AEAD.wgetinfo aw in
+  match AEAD.wentry_for_nonce #i n aw h with
+    | Some e ->
+      lemma_find_l_contains (AEAD.nonce_filter #i #aw n) awlg;
+      Seq.contains_elim awlg e;
+      create_nonce_inj'' i iv (U32.uint_to_t j)
+    | None -> Seq.find_l_none_no_index awlg (AEAD.nonce_filter #i #aw n);
+      assert (AEAD.nonce_filter #i #aw n (Seq.index awlg j))
+
+val lem_nonce3 (i:I.id) (w:stream_writer i) (j:nat) (h:mem) :
+  Lemma
+  (requires safeId i /\ invariant w h)
+  (ensures
+    j < wctrT w h ==> 
+    (let wlg = wlog w h in
+    let aw = Stream_writer?.aead w in
+    let awlg = AEAD.wlog aw h in
+    let n = create_nonce (Stream_writer?.iv w) (U32.uint_to_t j) in
+    let u = AEAD.wgetinfo aw in
+    match Seq.index wlg j with
+      | Entry ad #lmax p c ->
+        Some? (AEAD.wentry_for_nonce #i n aw h) /\
+       (match Some?.v (AEAD.wentry_for_nonce #i n aw h) with
+          | AEAD.Entry n' ad' #l p' c' ->
+        n' = n /\
+        ad' = ad /\
+        plain_of_aead_plain #i #l p' = p /\
+        cipher_of_aead_cipher c' = c /\
+        l = lmax + 1)))
+let lem_nonce3 i w j h = 
+  if j < wctrT w h then
+  begin
+  let wlg = wlog w h in
+  let aw = Stream_writer?.aead w in
+  let awlg = AEAD.wlog aw h in
+  let iv = Stream_writer?.iv w in
+  let n = create_nonce iv (U32.uint_to_t j) in
+  let u = AEAD.wgetinfo aw in
+  lem_nonce2 i w j h; lem_nonce i w j h
+  end
+
+val lem_nonce4 (i:I.id) (w:stream_writer i) (j:nat) (h:mem) :
+  Lemma
+  (requires safeId i /\ invariant w h /\ j <= wctrT w h)
+  (ensures
+    (let aw = Stream_writer?.aead w in
+    let n:AEAD.nonce i = create_nonce #i (Stream_writer?.iv w) (U32.uint_to_t j) in
+    Some? (AEAD.wentry_for_nonce #i n aw h) ==>
+    j < wctrT w h))
+let lem_nonce4 i w j h = 
+  let wlg = wlog w h in
+  let aw = Stream_writer?.aead w in
+  let awlg = AEAD.wlog aw h in
+  let iv = Stream_writer?.iv w in
+  let n = create_nonce iv (U32.uint_to_t j) in
+  let u = AEAD.wgetinfo aw in
+  match AEAD.wentry_for_nonce #i n aw h with
+    | Some e ->
+      lemma_find_l_contains (AEAD.nonce_filter #i #aw n) awlg;
+      Seq.contains_elim awlg e;
+      create_nonce_inj'' i iv (U32.uint_to_t j)
+    | None -> ()
+
+
+//#reset-options "--initial_fuel 2 --max_fuel 2 --z3rlimit 50"
+
+let decrypt #i (#w:stream_writer i) (r:stream_reader w) ad lmax (c:cipher i lmax) 
+=
+  let h0 = get() in
+  let aw = Stream_writer?.aead w in
   let ar = Stream_reader?.aead r in
+  assume (Set.disjoint (Set.singleton (AEAD.rgetinfo ar).AEAD.prf_rgn) (AEAD.wfootprint aw));
   let cc:AEAD.cipher i (AEAD.rgetinfo ar) (lmax+1) = aead_cipher_of_cipher (AEAD.rgetinfo ar) c in
   let ctr = (Stream_reader?.ctr r) in
   let n = create_nonce (Stream_reader?.iv r) !ctr in
   let op = AEAD.decrypt i ar ad n (lmax+1) cc in
-  admit();
+  let h05 = get() in
+  assume (
+    let s = (Set.union (AEAD.rfootprint ar) AEAD.shared_footprint) in
+    let ctr' = Stream_writer?.ctr w in
+    (~(Set.mem (frameOf ctr') s) /\ modifies s h0 h05) ==>
+
+    sel h0 ctr' == sel h05 ctr');
+  assume (
+    let s = (Set.union (AEAD.rfootprint ar) AEAD.shared_footprint) in
+    let ctr' = Stream_reader?.ctr r in
+    (~(Set.mem (frameOf ctr') s) /\ modifies s h0 h05) ==>
+    sel h0 ctr' == sel h05 ctr');
+//  assert (AEAD.winvariant aw h05);
+//  assert (wctrT w h05 == wctrT w h0);
+//  assert (rctrT r h05 == rctrT r h0);
+  if safeId i then aead_frame_log'' aw h0 (Set.union (AEAD.rfootprint ar) AEAD.shared_footprint) h05;
+//  assert (safeId i ==> AEAD.wlog aw h0 == AEAD.wlog aw h05);
+//  assert (invariant w h05);
+  if safeId i then lem_nonce3 i w (rctrT r h0) h0;
   match op with
-    | Some (pp:aead_plain i (lmax+1)) -> ctr := !ctr + 1; Some (unpad pp)
+    | Some (pp:aead_plain i (lmax+1)) ->
+      if safeId i then lem_nonce4 i w (rctrT r h0) h0;
+      ctr := !ctr +^ 1ul; 
+      let h1 = get() in 
+      assert (~ (Set.mem (Stream_reader?.region r) (AEAD.wfootprint aw)));
+      assert (~ (Set.mem (Stream_reader?.region r) (Set.singleton (Stream_writer?.region w))));
+      assert (~ (Set.mem (Stream_reader?.region r) (Set.union (AEAD.wfootprint aw) (Set.singleton (Stream_writer?.region w)))));
+      assert (~(Set.mem (Stream_reader?.region r) (footprint w)));
+      AEAD.wframe_invariant aw h05 (Stream_reader?.region r) h1;
+      frame_invariant w h05 (Stream_reader?.region r) h1;
+      if safeId i then
+        AEAD.frame_log aw (AEAD.wlog aw h05) h05 (Stream_reader?.region r) h1;
+      Some (unpad pp)
     | None -> None
